more proofs, but cannot work as is
The problem is that we have to handle new units that appear during
inprocessing. There are two ways to achieve that:
  - not doing by no taking care of binary clauses
  - properly removing units (which technically also mean that our
  single-watched-list can become wrong, which in turn is going to be
  an issue for the length of the clause)

The proper fix is probably to not handle binary clauses and have a
seperate pass just for them.

Weidenbach_Book/Watched_Literals/Watched_Literals_List_Inprocessing.thy
@@ -2036,28 +2036,41 @@ lemma subsume_or_strengthen:
   done
 
 definition forward_subsumption_one_inv :: \<open>nat \<Rightarrow> 'v twl_st_l \<Rightarrow> _ \<Rightarrow> bool\<close> where
-  \<open>forward_subsumption_one_inv = (\<lambda>C (M, N, D, NE, UE, NEk, UEk, NS, US, N0, U0, WS, Q) (xs, s).
-  subsume_or_strengthen_pre C s (M, N, D, NE, UE, NEk, UEk, NS, US, N0, U0, WS, Q) \<and> 
-    C \<notin># xs)\<close>
+  \<open>forward_subsumption_one_inv = (\<lambda>C S (T, xs, s).
+  (\<exists>S' . (S, S') \<in> twl_st_l None \<and>
+      twl_struct_invs S' \<and>
+      cdcl\<^sub>W_restart_mset.cdcl\<^sub>W_learned_clauses_entailed_by_init (state\<^sub>W_of S') \<and>
+    subsume_or_strengthen_pre C s T \<and>
+    C \<notin># xs \<and> C \<in># dom_m (get_clauses_l T) \<and> count_decided (get_trail_l S) = 0 \<and> 
+    clauses_to_update_l S = {#} \<and> twl_list_invs S \<and> twl_struct_invs S' \<and>
+   set (get_all_mark_of_propagated (get_trail_l S)) \<subseteq> {0} \<and>
+   cdcl\<^sub>W_restart_mset.cdcl\<^sub>W_learned_clauses_entailed_by_init (state\<^sub>W_of S') \<and>
+   cdcl_twl_inprocessing_l\<^sup>*\<^sup>* S T))\<close>
 
-definition forward_subsumption_one :: \<open>nat \<Rightarrow> 'v twl_st_l \<Rightarrow> ('v twl_st_l \<times> bool) nres\<close> where
-  \<open>forward_subsumption_one = (\<lambda>C (M, N, D, NE, UE, NEk, UEk, NS, US, N0, U0, WS, Q) . do {
-  ASSERT(forward_subsumption_one_pre C (M, N, D, NE, UE, NEk, UEk, NS, US, N0, U0, WS, Q));
-  xs \<leftarrow> SPEC (\<lambda>xs. C \<notin># xs);
-  (xs, s) \<leftarrow>
-    WHILE\<^sub>T\<^bsup> forward_subsumption_one_inv C (M, N, D, NE, UE, NEk, UEk, NS, US, N0, U0, WS, Q) \<^esup> (\<lambda>(xs, s). xs \<noteq> {#} \<and> s = NONE)
-    (\<lambda>(xs, s). do {
-      C' \<leftarrow> SPEC(\<lambda>C'. C' \<in># xs);
-      if C' \<notin># dom_m N
-      then RETURN (remove1_mset C' xs, s)
-      else do  {
-        s \<leftarrow> SPEC(try_to_subsume C C' N);
-       RETURN (remove1_mset C' xs, s)
-      }
-    })
-    (xs, NONE);
-  S \<leftarrow> subsume_or_strengthen C s (M, N, D, NE, UE, NEk, UEk, NS, US, N0, U0, WS, Q);
-  RETURN (S, s \<noteq> NONE)
+
+definition forward_subsumption_one :: \<open> nat \<Rightarrow> 'v twl_st_l \<Rightarrow> ('v twl_st_l \<times> bool) nres\<close> where
+  \<open>forward_subsumption_one = (\<lambda>C S . do {
+    ASSERT(forward_subsumption_one_pre C S);
+    xs \<leftarrow> SPEC (\<lambda>xs. C \<notin># xs);
+    (S, xs, s) \<leftarrow>
+      WHILE\<^sub>T\<^bsup> forward_subsumption_one_inv C S \<^esup> (\<lambda>(S, xs, s). xs \<noteq> {#} \<and> s = NONE \<and> get_conflict_l S = None)
+      (\<lambda>(S, xs, s). do {
+        C' \<leftarrow> SPEC(\<lambda>C'. C' \<in># xs);
+        if C' \<notin># dom_m (get_clauses_l S) 
+        then RETURN (S, remove1_mset C' xs, s)
+        else do {
+          S \<leftarrow> simplify_clause_with_unit_st C' S;
+          if C' \<notin># dom_m (get_clauses_l S) \<or> get_conflict_l S \<noteq> None
+          then RETURN (S, remove1_mset C' xs, s)
+          else do  {
+            s \<leftarrow> SPEC(try_to_subsume C C' (get_clauses_l S));
+           RETURN (S, remove1_mset C' xs, s)
+          }
+        }
+      })
+      (S, xs, NONE);
+    S \<leftarrow> subsume_or_strengthen C s S;
+    RETURN (S, s \<noteq> NONE)
   }
 )\<close>
 
@@ -2068,83 +2081,6 @@ lemma subset_mset_removeAll_iff:
     count_le_replicate_mset_subset_eq diff_subset_eq_self diff_zero filter_union_mset insert_iff
     mset_le_subtract_right removeAll_mset_filter_mset replicate_mset_minus_replicate_mset_same
     replicate_mset_subseteq_iff_le set_mset_minus_replicate_mset(1) subset_mset.diff_add)
-
-lemma forward_subsumption_one:
-  assumes \<open>forward_subsumption_one_pre C S\<close>
-  shows \<open>forward_subsumption_one C S \<le> \<Down>{((st, SR), st'). st = st' \<and> (\<not>SR \<longrightarrow> st = S)} (SPEC(cdcl_twl_inprocessing_l\<^sup>*\<^sup>* S))\<close>
-proof -
-  obtain x where
-    Sx: \<open>(S, x) \<in> twl_st_l None\<close> and
-    struct: \<open>twl_struct_invs x\<close> and
-    st_inv: \<open>twl_st_inv x\<close> and
-    list_invs: \<open>twl_list_invs S\<close> and
-    C: \<open>C \<in># dom_m (get_clauses_l S)\<close> and
-    \<open>cdcl\<^sub>W_restart_mset.cdcl\<^sub>W_all_struct_inv (state\<^sub>W_of x)\<close> and
-    clss: \<open>clauses_to_update_l S = {#}\<close> \<open>get_conflict_l S = None\<close> and
-    no_annot: \<open>set (get_all_mark_of_propagated (get_trail_l S)) \<subseteq> {0}\<close>
-    using assms unfolding forward_subsumption_one_pre_def twl_struct_invs_def
-      pcdcl_all_struct_invs_def state\<^sub>W_of_def
-    apply -
-    by normalize_goal+ blast
-  have [refine0]: \<open>wf (measure (\<lambda>(d, _). size d))\<close>
-    by auto
-  have H: \<open>length (get_clauses_l S \<propto> D) \<ge>2\<close> \<open>distinct (get_clauses_l S \<propto> D)\<close>  \<open>D \<noteq> 0\<close>
-    \<open>D \<notin> set (get_all_mark_of_propagated (get_trail_l S))\<close> if \<open>D \<in># dom_m (get_clauses_l S)\<close>for D
-    using st_inv that Sx list_invs no_annot unfolding twl_struct_invs_def twl_list_invs_def apply -
-    by (auto simp: twl_struct_invs_def twl_st_l_def ran_m_def conj_disj_distribR
-      twl_st_inv.simps Collect_disj_eq image_image image_Un Collect_conv_if mset_take_mset_drop_mset'
-      dest!: multi_member_split split: if_splits
-      simp flip: insert_compr)
-  have H2: \<open>\<not>tautology (mset (get_clauses_l S \<propto> D))\<close> if \<open>D \<in># dom_m (get_clauses_l S)\<close> for D
-    using list_invs that by (auto simp: twl_list_invs_def ran_m_def)
-
-  show ?thesis
-    unfolding forward_subsumption_one_def conc_fun_RES
-    apply (rewrite at \<open>_ \<le> \<hole>\<close> RES_SPEC_conv)
-    apply (refine_vcg subsume_or_strengthen[unfolded Down_id_eq])
-    subgoal using assms by auto
-    subgoal
-      using H by (auto simp: subsume_or_strengthen_pre_def
-      forward_subsumption_one_pre_def distinct_mset_dom distinct_mset_remove1_All
-       forward_subsumption_one_inv_def subset_mset_removeAll_iff split)
-    subgoal by (auto simp: forward_subsumption_one_inv_def dest: in_diffD)
-    subgoal by (auto simp: forward_subsumption_one_inv_def dest: multi_member_split)
-    subgoal for a b aa ba ab bb ac bc ad bd ae be af bf ag bg ah bh ai bi aj bj ak bk x s al bl xa xb
-      using H C H2 not_tautology_mono[of \<open>mset (removeAll _ (get_clauses_l S \<propto> C))\<close>
-        \<open>mset (get_clauses_l S \<propto> C)\<close>]
-      apply (auto simp: try_to_subsume_def distinct_mset_dom distinct_mset_remove1_All
-        subsume_or_strengthen_pre_def subset_mset_removeAll_iff tautology_union
-        forward_subsumption_one_inv_def
-        simp del: mset_removeAll
-        simp flip: mset_removeAll
-        split: subsumption.splits
-        dest: in_diffD)[]
-       apply (metis subset_mset.diff_add tautology_union)
-       by (smt (z3) count_le_replicate_mset_subset_eq in_replicate_mset order_refl set_mset_mset subset_mset.diff_add tautology_minus union_iff)
-    subgoal
-      by (auto dest!: multi_member_split)
-    subgoal
-      unfolding forward_subsumption_one_inv_def by blast
-    subgoal unfolding forward_subsumption_one_pre_def by auto
-    subgoal using clss by (auto simp only:)
-    done
-qed
-
-definition simplify_clauses_with_unit_st_pre where
-  \<open>simplify_clauses_with_unit_st_pre S \<longleftrightarrow> (\<exists>T.
-  (S, T) \<in> twl_st_l None \<and>
-  twl_struct_invs T \<and>
-  twl_list_invs S \<and>
-  clauses_to_update_l S = {#} \<and>
-  cdcl\<^sub>W_restart_mset.cdcl\<^sub>W_learned_clauses_entailed_by_init (state\<^sub>W_of T) \<and>
-  count_decided (get_trail_l S) = 0 \<and>
-  set (get_all_mark_of_propagated (get_trail_l S)) \<subseteq> {0})\<close>
-
-definition simplify_clauses_with_unit_st_inv :: \<open>'v twl_st_l \<Rightarrow> nat set \<Rightarrow> 'v twl_st_l \<Rightarrow> bool\<close> where
-  \<open>simplify_clauses_with_unit_st_inv S\<^sub>0 it S \<longleftrightarrow> (
-    cdcl_twl_inprocessing_l\<^sup>*\<^sup>* S\<^sub>0 S \<and>
-  set (get_all_mark_of_propagated (get_trail_l S)) \<subseteq>
-    set (get_all_mark_of_propagated (get_trail_l S\<^sub>0)) \<union> {0})\<close>
 
 lemma cdcl_twl_inprocessing_l_twl_st_l0:
   assumes \<open>cdcl_twl_inprocessing_l S U\<close> and
@@ -2169,6 +2105,7 @@ lemma cdcl_twl_unitres_l_list_invs:
     ran_m_mapsto_upd
     dest: in_diffD)
 
+
 lemma cdcl_twl_inprocessing_l_twl_list_invs:
   assumes \<open>cdcl_twl_inprocessing_l S U\<close> and
     \<open>twl_list_invs S\<close>
@@ -2187,6 +2124,7 @@ lemma rtranclp_cdcl_twl_inprocessing_l_twl_list_invs:
   using assms by (induction rule: rtranclp_induct)
     (auto simp: cdcl_twl_inprocessing_l_twl_list_invs)
  
+
 lemma cdcl_twl_inprocessing_l_twl_st_l:
   assumes \<open>cdcl_twl_inprocessing_l S U\<close> and
     \<open>(S, T) \<in> twl_st_l None\<close> and
@@ -2213,6 +2151,7 @@ lemma cdcl_twl_inprocessing_l_twl_st_l:
     done
   done
 
+
 lemma rtranclp_cdcl_twl_inprocessing_l_twl_st_l:
   assumes \<open>cdcl_twl_inprocessing_l\<^sup>*\<^sup>* S U\<close> and
     \<open>(S, T) \<in> twl_st_l None\<close> and
@@ -2234,6 +2173,297 @@ lemma rtranclp_cdcl_twl_inprocessing_l_twl_st_l:
     apply assumption+
     done
   done
+
+
+lemma
+  assumes \<open>cdcl_twl_inprocessing_l\<^sup>*\<^sup>* S T\<close>
+  shows
+    rtranclp_cdcl_twl_inprocessing_l_count_decided:
+    \<open>count_decided (get_trail_l T) = count_decided (get_trail_l S)\<close> (is ?A) and
+    rtranclp_cdcl_twl_inprocessing_l_clauses_to_update_l:
+    \<open>clauses_to_update_l T = clauses_to_update_l S\<close> (is ?B) and
+    rtranclp_cdcl_twl_inprocessing_l_get_all_mark_of_propagated:
+    \<open>set (get_all_mark_of_propagated (get_trail_l T)) \<subseteq> set (get_all_mark_of_propagated (get_trail_l S)) \<union> {0}\<close> (is ?C)
+proof -
+  have [dest]:
+    \<open>cdcl_twl_inprocessing_l S T \<Longrightarrow> count_decided (get_trail_l T) = count_decided (get_trail_l S)\<close> 
+    \<open>cdcl_twl_inprocessing_l S T \<Longrightarrow> clauses_to_update_l T = clauses_to_update_l S\<close>
+    \<open>cdcl_twl_inprocessing_l S T \<Longrightarrow> set (get_all_mark_of_propagated (get_trail_l T)) \<subseteq> set (get_all_mark_of_propagated (get_trail_l S)) \<union> {0}\<close> for S T
+    by (auto simp: cdcl_twl_inprocessing_l.simps cdcl_twl_subsumed_l.simps
+      cdcl_twl_unitres_l.simps cdcl_twl_subresolution_l.simps cdcl_twl_unitres_true_l.simps)
+      (*set (get_all_mark_of_propagated (get_trail_l T))*)
+  show ?A ?B ?C
+    using assms
+    by (induction rule: rtranclp_induct; auto; fail)+
+qed
+
+lemma forward_subsumption_one_inv_alt_def:
+  \<open>forward_subsumption_one_inv = (\<lambda>C S (T, xs, s).
+  (\<exists>S' T'. (S, S') \<in> twl_st_l None \<and>
+      twl_struct_invs S' \<and>
+      cdcl\<^sub>W_restart_mset.cdcl\<^sub>W_learned_clauses_entailed_by_init (state\<^sub>W_of S') \<and>
+    subsume_or_strengthen_pre C s T \<and>
+    C \<notin># xs \<and> C \<in># dom_m (get_clauses_l T) \<and> count_decided (get_trail_l S) = 0 \<and> 
+    clauses_to_update_l S = {#} \<and> twl_list_invs S \<and> twl_struct_invs S' \<and>
+   set (get_all_mark_of_propagated (get_trail_l S)) \<subseteq> {0} \<and>
+   cdcl\<^sub>W_restart_mset.cdcl\<^sub>W_learned_clauses_entailed_by_init (state\<^sub>W_of S') \<and>
+   (T, T') \<in> twl_st_l None \<and>
+      twl_struct_invs T' \<and>
+      cdcl\<^sub>W_restart_mset.cdcl\<^sub>W_learned_clauses_entailed_by_init (state\<^sub>W_of T') \<and>
+    C \<notin># xs \<and> C \<in># dom_m (get_clauses_l T) \<and> count_decided (get_trail_l T) = 0 \<and> 
+    clauses_to_update_l T = {#} \<and> twl_list_invs T \<and> twl_struct_invs T' \<and>
+   set (get_all_mark_of_propagated (get_trail_l T)) \<subseteq> {0} \<and>
+   cdcl\<^sub>W_restart_mset.cdcl\<^sub>W_learned_clauses_entailed_by_init (state\<^sub>W_of T') \<and>
+   cdcl_twl_inprocessing_l\<^sup>*\<^sup>* S T))\<close>
+  unfolding forward_subsumption_one_inv_def
+  apply (rule iffI ext)+
+  apply (case_tac x; hypsubst)
+  unfolding prod.simps
+  apply normalize_goal+
+  apply (frule rtranclp_cdcl_twl_inprocessing_l_twl_st_l; assumption?)
+  apply (rule_tac x=xa in exI)
+  apply (rule_tac x=V in exI)
+  apply (simp add: rtranclp_cdcl_twl_inprocessing_l_count_decided
+   rtranclp_cdcl_twl_inprocessing_l_clauses_to_update_l rtranclp_cdcl_twl_inprocessing_l_get_all_mark_of_propagated)
+  apply (drule rtranclp_cdcl_twl_inprocessing_l_get_all_mark_of_propagated, blast)
+  apply (case_tac x; hypsubst)
+  unfolding prod.simps
+  apply normalize_goal+
+  apply (frule rtranclp_cdcl_twl_inprocessing_l_twl_st_l; assumption?)
+  apply (rule_tac x=xa in exI)
+  apply simp
+  done
+
+
+lemma forward_subsumption_one:
+  assumes \<open>forward_subsumption_one_pre C S\<close>
+  shows \<open>forward_subsumption_one C S \<le> \<Down>{((st, SR), st'). st = st' \<and> (\<not>SR \<longrightarrow> st = S)} (SPEC(cdcl_twl_inprocessing_l\<^sup>*\<^sup>* S))\<close>
+proof -
+  obtain x where
+    Sx: \<open>(S, x) \<in> twl_st_l None\<close> and
+    struct: \<open>twl_struct_invs x\<close> and
+    st_inv: \<open>twl_st_inv x\<close> and
+    list_invs: \<open>twl_list_invs S\<close> and
+    C: \<open>C \<in># dom_m (get_clauses_l S)\<close> and
+    \<open>cdcl\<^sub>W_restart_mset.cdcl\<^sub>W_all_struct_inv (state\<^sub>W_of x)\<close> and
+    clss: \<open>clauses_to_update_l S = {#}\<close> \<open>get_conflict_l S = None\<close> and
+    no_annot: \<open>set (get_all_mark_of_propagated (get_trail_l S)) \<subseteq> {0}\<close> and
+    init: \<open>cdcl\<^sub>W_restart_mset.cdcl\<^sub>W_learned_clauses_entailed_by_init (state\<^sub>W_of x)\<close> and
+    dec: \<open>count_decided (get_trail_l S) = 0\<close>
+    using assms unfolding forward_subsumption_one_pre_def twl_struct_invs_def
+      pcdcl_all_struct_invs_def state\<^sub>W_of_def
+    apply -
+    by normalize_goal+ blast
+  have [refine0]: \<open>wf (measure (\<lambda>(_, d, _). size d))\<close>
+    by auto
+  have H: \<open>length (get_clauses_l S \<propto> D) \<ge>2\<close> \<open>distinct (get_clauses_l S \<propto> D)\<close>  \<open>D \<noteq> 0\<close>
+    \<open>D \<notin> set (get_all_mark_of_propagated (get_trail_l S))\<close> if \<open>D \<in># dom_m (get_clauses_l S)\<close>for D
+    using st_inv that Sx list_invs no_annot unfolding twl_struct_invs_def twl_list_invs_def apply -
+    by (auto simp: twl_struct_invs_def twl_st_l_def ran_m_def conj_disj_distribR
+      twl_st_inv.simps Collect_disj_eq image_image image_Un Collect_conv_if mset_take_mset_drop_mset'
+      dest!: multi_member_split split: if_splits
+      simp flip: insert_compr)
+  have H2: \<open>\<not>tautology (mset (get_clauses_l S \<propto> D))\<close> if \<open>D \<in># dom_m (get_clauses_l S)\<close> for D
+    using list_invs that by (auto simp: twl_list_invs_def ran_m_def)
+find_theorems simplify_clause_with_unit_st
+
+  have \<open>subsume_or_strengthen_pre C (snd (snd xb')) U\<close>
+    if 
+      \<open>forward_subsumption_one_pre C S\<close> and
+      \<open>C \<notin># xs\<close> and
+      \<open>xa \<in># b\<close> and
+      \<open>xa \<in># dom_m (get_clauses_l ab)\<close> and
+      \<open>xa \<in># dom_m (get_clauses_l U) \<and> get_conflict_l U = None\<close> and
+      xb': \<open>xb'
+    \<in> (\<lambda>x. (U, remove1_mset xa b, x)) `
+      Collect (try_to_subsume C xa (get_clauses_l U))\<close> and
+      \<open>s = (ab, b, NONE)\<close> and
+      \<open>ba' = (b, NONE)\<close> and
+      \<open>b \<noteq> {#}\<close> and
+      abU: \<open>ab = U \<or> cdcl_twl_unitres_l ab U \<or> cdcl_twl_unitres_true_l ab U\<close> and
+      \<open>a = ab\<close> and
+      \<open>(S, x) \<in> twl_st_l None\<close> and
+      \<open>c = NONE\<close> and
+      \<open>get_conflict_l ab = None\<close> and
+      \<open>set (get_all_mark_of_propagated (get_trail_l U))
+    \<subseteq> insert 0 (set (get_all_mark_of_propagated (get_trail_l ab)))\<close> and
+      \<open>aa = b\<close> and
+      \<open>ba = NONE\<close> and
+      dom_U: \<open>dom_m (get_clauses_l U) = dom_m (get_clauses_l ab) \<or>
+    dom_m (get_clauses_l U) = remove1_mset xa (dom_m (get_clauses_l ab))\<close> and
+      all_undef: \<open>\<forall>L\<in>set (get_clauses_l U \<propto> xa). undefined_lit (get_trail_l U) L\<close> and
+      \<open>cdcl\<^sub>W_restart_mset.cdcl\<^sub>W_learned_clauses_entailed_by_init
+     (state_of (pstate\<^sub>W_of x))\<close> and
+      \<open>subsume_or_strengthen_pre C NONE S\<close> and
+      \<open>C \<notin># b\<close> and
+      \<open>C \<in># dom_m (get_clauses_l ab)\<close> and
+      \<open>count_decided (get_trail_l S) = 0\<close> and
+      \<open>clauses_to_update_l S = {#}\<close> and
+      \<open>twl_list_invs S\<close> and
+      \<open>twl_struct_invs x\<close> and
+      \<open>set (get_all_mark_of_propagated (get_trail_l S)) \<subseteq> {0}\<close> and
+      ST: \<open>cdcl_twl_inprocessing_l\<^sup>*\<^sup>* S ab\<close>
+    for ab U xa c xb xb' ba'
+  proof -
+    have C_ab: \<open>C \<in># dom_m (get_clauses_l ab)\<close>
+      using that by simp_all
+    have SU: \<open>cdcl_twl_inprocessing_l\<^sup>*\<^sup>* S U\<close>
+      using ST abU by (auto dest!: cdcl_twl_inprocessing_l.intros)
+    have no_annot: \<open>set (get_all_mark_of_propagated (get_trail_l U)) \<subseteq> {0}\<close> and
+      dec: \<open>count_decided (get_trail_l U) = 0\<close>
+      using \<open>set (get_all_mark_of_propagated (get_trail_l S)) \<subseteq> {0}\<close>
+        rtranclp_cdcl_twl_inprocessing_l_get_all_mark_of_propagated[OF SU]
+        rtranclp_cdcl_twl_inprocessing_l_count_decided[OF SU]
+      unfolding \<open>count_decided (get_trail_l S) = 0\<close>
+      by blast+
+    obtain x where
+      Sx: \<open>(U, x) \<in> twl_st_l None\<close> and
+      struct: \<open>twl_struct_invs x\<close> and
+      list_invs: \<open>twl_list_invs U\<close> and
+      init: \<open>cdcl\<^sub>W_restart_mset.cdcl\<^sub>W_learned_clauses_entailed_by_init (state\<^sub>W_of x)\<close>
+      subgoal premises p
+        by (rule rtranclp_cdcl_twl_inprocessing_l_twl_st_l[OF SU Sx struct list_invs init])
+         (rule that; (assumption)?)
+      done
+    have \<open>cdcl\<^sub>W_restart_mset.cdcl\<^sub>W_all_struct_inv (state\<^sub>W_of x)\<close> and
+      st_inv: \<open>twl_st_inv x\<close>
+      using struct
+      unfolding forward_subsumption_one_pre_def twl_struct_invs_def
+        pcdcl_all_struct_invs_def state\<^sub>W_of_def by fast+
+    have C: \<open>C \<in># dom_m (get_clauses_l U)\<close>
+      using dom_U C_ab that(3,5,22) by (auto intro!: in_remove1_msetI)
+    have H: \<open>length (get_clauses_l U \<propto> D) \<ge>2\<close> \<open>distinct (get_clauses_l U \<propto> D)\<close>  \<open>D \<noteq> 0\<close>
+      \<open>D \<notin> set (get_all_mark_of_propagated (get_trail_l U))\<close> if \<open>D \<in># dom_m (get_clauses_l U)\<close>for D
+      using st_inv that Sx list_invs no_annot unfolding twl_struct_invs_def twl_list_invs_def apply -
+      by (auto simp: twl_struct_invs_def twl_st_l_def ran_m_def conj_disj_distribR
+        twl_st_inv.simps Collect_disj_eq image_image image_Un Collect_conv_if mset_take_mset_drop_mset'
+        dest!: multi_member_split split: if_splits
+        simp flip: insert_compr)
+    show ?thesis
+      using H C xb' dec all_undef unfolding subsume_or_strengthen_pre_def try_to_subsume_def
+      apply (case_tac x)
+      apply (auto split: subsumption.splits simp add: state_decomp_to_state_l) sorry
+  qed
+
+  show ?thesis
+    unfolding forward_subsumption_one_def conc_fun_RES
+    apply (rewrite at \<open>_ \<le> \<hole>\<close> RES_SPEC_conv)
+    apply (refine_vcg subsume_or_strengthen[unfolded Down_id_eq]
+      simplify_clause_with_unit_st_spec[THEN order_trans] if_rule)
+    subgoal using assms by auto
+    subgoal for ax
+      unfolding forward_subsumption_one_inv_def prod.simps
+      apply (rule_tac x=x in exI)
+      using Sx H struct st_inv C init by (auto simp add: subsume_or_strengthen_pre_def forward_subsumption_one_pre_def)
+   subgoal for xs
+     unfolding simplify_clause_with_unit_st_pre_def forward_subsumption_one_inv_def case_prod_beta
+     apply normalize_goal+ 
+     by (rule_tac x=x in exI)
+      (auto dest: in_diffD)
+   subgoal
+     unfolding simplify_clause_with_unit_st_pre_def forward_subsumption_one_inv_def case_prod_beta
+     apply normalize_goal+ 
+     by  (auto dest: multi_member_split)
+   subgoal
+     unfolding simplify_clause_with_unit_st_pre_def forward_subsumption_one_inv_alt_def case_prod_beta
+     apply normalize_goal+ 
+    apply (intro conjI)
+    apply ((solves \<open>use dec init C in \<open>simp\<close>\<close>))+
+    apply ((solves \<open>use dec init C in \<open>fastforce\<close>\<close>)?)
+    done
+
+   subgoal for xs s a b aa ba xa unfolding Down_id_eq
+     apply (intro SPEC_rule)
+     apply (rule if_rule)
+     subgoal
+       apply clarsimp
+       apply (intro conjI)
+       subgoal
+         unfolding forward_subsumption_one_inv_def prod.simps
+         apply normalize_goal+
+         apply (rule_tac x=x in exI)
+         apply simp
+        apply (intro conjI)
+        defer
+        apply (metis in_diffD) 
+        apply (metis in_remove1_msetI)
+        apply (auto dest!: cdcl_twl_inprocessing_l.intros)
+        done
+     subgoal by (auto dest!: multi_member_split)
+     done
+   subgoal for U
+     unfolding RES_RETURN_RES
+     apply (subst nres_order_simps)
+     apply rule
+     apply (subst mem_Collect_eq)
+     apply (intro conjI)
+     subgoal for x
+        apply (case_tac s, hypsubst)
+         unfolding forward_subsumption_one_inv_def prod.simps case_prod_beta
+         apply normalize_goal+
+         apply (rule_tac x=x in exI)
+         apply simp
+         apply (intro conjI)
+defer
+       apply (clarsimp dest!: in_diffD)
+       apply (auto dest!: in_diffD intro: in_remove1_msetI)[]
+       apply (auto dest!: cdcl_twl_inprocessing_l.intros)[]
+explore_have
+find_theorems subsume_or_strengthen_pre 
+ apply simp
+     apply rule
+     apply simp
+     apply (intro conjI impI)
+     apply normalize_goal+
+    
+
+       find_theorems "SPEC _ \<le> SPEC _"
+oops
+      using H by (auto simp: subsume_or_strengthen_pre_def
+      forward_subsumption_one_pre_def distinct_mset_dom distinct_mset_remove1_All
+       forward_subsumption_one_inv_def subset_mset_removeAll_iff split)
+    subgoal 
+      unfolding simplify_clause_with_unit_st_pre_def
+ sorry
+    subgoal by (auto simp: forward_subsumption_one_inv_def dest: in_diffD)
+    subgoal by (auto simp: forward_subsumption_one_inv_def dest: multi_member_split)
+    subgoal for a b aa ba ab bb ac bc ad bd ae be af bf ag bg ah bh ai bi aj bj ak bk x s al bl xa xb
+      using H C H2 not_tautology_mono[of \<open>mset (removeAll _ (get_clauses_l S \<propto> C))\<close>
+        \<open>mset (get_clauses_l S \<propto> C)\<close>]
+      apply (auto simp: try_to_subsume_def distinct_mset_dom distinct_mset_remove1_All
+        subsume_or_strengthen_pre_def subset_mset_removeAll_iff tautology_union
+        forward_subsumption_one_inv_def
+        simp del: mset_removeAll
+        simp flip: mset_removeAll
+        split: subsumption.splits
+        dest: in_diffD)[]
+       apply (metis subset_mset.diff_add tautology_union)
+       by (smt (z3) count_le_replicate_mset_subset_eq in_replicate_mset order_refl set_mset_mset subset_mset.diff_add tautology_minus union_iff)
+    subgoal
+      by (auto dest!: multi_member_split)
+    subgoal
+      unfolding forward_subsumption_one_inv_def by blast
+    subgoal unfolding forward_subsumption_one_pre_def by auto
+    subgoal using clss apply (auto simp only:)
+      sorry
+    done
+qed
+
+definition simplify_clauses_with_unit_st_pre where
+  \<open>simplify_clauses_with_unit_st_pre S \<longleftrightarrow> (\<exists>T.
+  (S, T) \<in> twl_st_l None \<and>
+  twl_struct_invs T \<and>
+  twl_list_invs S \<and>
+  clauses_to_update_l S = {#} \<and>
+  cdcl\<^sub>W_restart_mset.cdcl\<^sub>W_learned_clauses_entailed_by_init (state\<^sub>W_of T) \<and>
+  count_decided (get_trail_l S) = 0 \<and>
+  set (get_all_mark_of_propagated (get_trail_l S)) \<subseteq> {0})\<close>
+
+definition simplify_clauses_with_unit_st_inv :: \<open>'v twl_st_l \<Rightarrow> nat set \<Rightarrow> 'v twl_st_l \<Rightarrow> bool\<close> where
+  \<open>simplify_clauses_with_unit_st_inv S\<^sub>0 it S \<longleftrightarrow> (
+    cdcl_twl_inprocessing_l\<^sup>*\<^sup>* S\<^sub>0 S \<and>
+  set (get_all_mark_of_propagated (get_trail_l S)) \<subseteq>
+    set (get_all_mark_of_propagated (get_trail_l S\<^sub>0)) \<union> {0})\<close>
 
 lemma simplify_clauses_with_unit_st_inv_simplify_clauses_with_unit_st_preD:
   assumes
@@ -2492,15 +2722,16 @@ lemma simplify_clauses_with_units_st_spec:
   subgoal unfolding simplify_clauses_with_unit_st_inv_def by auto
   done
 
-definition try_to_forward_subsume_inv :: \<open>'v twl_st_l \<Rightarrow> nat \<Rightarrow> nat \<times> bool \<times> 'v twl_st_l \<Rightarrow> bool\<close> where
-  \<open>try_to_forward_subsume_inv S0 = (\<lambda>C (i,brk,S).
+definition try_to_forward_subsume_inv :: \<open>bool \<Rightarrow> 'v twl_st_l \<Rightarrow> nat \<Rightarrow> nat \<times> bool \<times> 'v twl_st_l \<Rightarrow> bool\<close> where
+  \<open>try_to_forward_subsume_inv no_bin S0 = (\<lambda>C (i,brk,S).
   (cdcl_twl_inprocessing_l\<^sup>*\<^sup>* S0 S \<and>
   clauses_to_update_l S = {#} \<and>
   count_decided (get_trail_l S) = 0 \<and>
   set (get_all_mark_of_propagated (get_trail_l S)) \<subseteq> {0} \<and>
   (\<not>brk \<longrightarrow> (get_conflict_l S = None \<and> C \<in># dom_m (get_clauses_l S) \<and>
   (\<forall>L \<in># mset (get_clauses_l S \<propto> C). undefined_lit (get_trail_l S) L) \<and>
-  length (get_clauses_l S \<propto> C) \<ge> 2))))\<close>
+  length (get_clauses_l S \<propto> C) \<ge> 2)) \<and>
+  (no_bin \<longrightarrow> get_trail_l S = get_trail_l S0)))\<close>
 
 definition try_to_forward_subsume_pre :: \<open>nat \<Rightarrow> 'v twl_st_l \<Rightarrow> bool\<close> where
   \<open>try_to_forward_subsume_pre = (\<lambda>C S.
@@ -2517,11 +2748,11 @@ definition try_to_forward_subsume_pre :: \<open>nat \<Rightarrow> 'v twl_st_l \<
   (\<forall>L \<in># mset (get_clauses_l S \<propto> C). undefined_lit (get_trail_l S) L) \<and>
   length (get_clauses_l S \<propto> C) \<ge> 2)\<close>
 
-definition try_to_forward_subsume :: \<open>nat \<Rightarrow> 'v twl_st_l \<Rightarrow> 'v twl_st_l nres\<close> where
-  \<open>try_to_forward_subsume C S = do {
+definition try_to_forward_subsume :: \<open>bool \<Rightarrow> nat \<Rightarrow> 'v twl_st_l \<Rightarrow> 'v twl_st_l nres\<close> where
+  \<open>try_to_forward_subsume no_bin C S = do {
   ASSERT (try_to_forward_subsume_pre C S);
   n \<leftarrow> RES {_::nat. True};
-  (_, _, S) \<leftarrow> WHILE\<^sub>T\<^bsup> try_to_forward_subsume_inv S C\<^esup>
+  (_, _, S) \<leftarrow> WHILE\<^sub>T\<^bsup> try_to_forward_subsume_inv no_bin S C\<^esup>
     (\<lambda>(i, break, S). \<not>break \<and> i < n)
     (\<lambda>(i, break, S). do {
       (S, subs) \<leftarrow> forward_subsumption_one C S;
@@ -2533,31 +2764,9 @@ definition try_to_forward_subsume :: \<open>nat \<Rightarrow> 'v twl_st_l \<Righ
   }
   \<close>
 
-lemma
-  assumes \<open>cdcl_twl_inprocessing_l\<^sup>*\<^sup>* S T\<close>
-  shows
-    rtranclp_cdcl_twl_inprocessing_l_count_decided:
-    \<open>count_decided (get_trail_l T) = count_decided (get_trail_l S)\<close> (is ?A) and
-    rtranclp_cdcl_twl_inprocessing_l_clauses_to_update_l:
-    \<open>clauses_to_update_l T = clauses_to_update_l S\<close> (is ?B) and
-    rtranclp_cdcl_twl_inprocessing_l_get_all_mark_of_propagated:
-    \<open>set (get_all_mark_of_propagated (get_trail_l T)) \<subseteq> set (get_all_mark_of_propagated (get_trail_l S)) \<union> {0}\<close> (is ?C)
-proof -
-  have [dest]:
-    \<open>cdcl_twl_inprocessing_l S T \<Longrightarrow> count_decided (get_trail_l T) = count_decided (get_trail_l S)\<close> 
-    \<open>cdcl_twl_inprocessing_l S T \<Longrightarrow> clauses_to_update_l T = clauses_to_update_l S\<close>
-    \<open>cdcl_twl_inprocessing_l S T \<Longrightarrow> set (get_all_mark_of_propagated (get_trail_l T)) \<subseteq> set (get_all_mark_of_propagated (get_trail_l S)) \<union> {0}\<close> for S T
-    by (auto simp: cdcl_twl_inprocessing_l.simps cdcl_twl_subsumed_l.simps
-      cdcl_twl_unitres_l.simps cdcl_twl_subresolution_l.simps cdcl_twl_unitres_true_l.simps)
-      (*set (get_all_mark_of_propagated (get_trail_l T))*)
-  show ?A ?B ?C
-    using assms
-    by (induction rule: rtranclp_induct; auto; fail)+
-qed
-
 lemma try_to_forward_forward_subsumption_one_pre:
   \<open>try_to_forward_subsume_pre C S \<Longrightarrow>
-  try_to_forward_subsume_inv S C (a, False, ba) \<Longrightarrow> forward_subsumption_one_pre C ba\<close>
+  try_to_forward_subsume_inv no_bin S C (a, False, ba) \<Longrightarrow> forward_subsumption_one_pre C ba\<close>
   unfolding try_to_forward_subsume_inv_def forward_subsumption_one_pre_def case_prod_beta
     try_to_forward_subsume_pre_def
   apply normalize_goal+
@@ -2569,7 +2778,7 @@ lemma try_to_forward_forward_subsumption_one_pre:
 
 lemma try_to_forward_subsume:
   assumes \<open>try_to_forward_subsume_pre C S\<close>
-  shows \<open>try_to_forward_subsume C S \<le> \<Down>Id (SPEC(cdcl_twl_inprocessing_l\<^sup>*\<^sup>* S))\<close>
+  shows \<open>try_to_forward_subsume no_bin C S \<le> \<Down>Id (SPEC(cdcl_twl_inprocessing_l\<^sup>*\<^sup>* S))\<close>
 proof -
   have wf: \<open>wf (measure (\<lambda>(i, _, _). Suc n - i))\<close> for n
     by auto
@@ -2605,8 +2814,8 @@ definition forward_subsumption_all_pre :: \<open>'v twl_st_l \<Rightarrow> bool\
 definition forward_subsumption_all_inv :: \<open>'v twl_st_l \<Rightarrow> nat multiset \<times> 'v twl_st_l \<Rightarrow> bool\<close> where
   \<open>forward_subsumption_all_inv S = (\<lambda>(xs, T). cdcl_twl_inprocessing_l\<^sup>*\<^sup>* S T \<and> xs \<subseteq># dom_m (get_clauses_l S))\<close>
 
-definition forward_subsumption_all :: \<open>'v twl_st_l \<Rightarrow> 'v twl_st_l nres\<close> where
-  \<open>forward_subsumption_all = (\<lambda>S. do {
+definition forward_subsumption_all :: \<open>bool \<Rightarrow> 'v twl_st_l \<Rightarrow> 'v twl_st_l nres\<close> where
+  \<open>forward_subsumption_all = (\<lambda>no_bin S. do {
   ASSERT (forward_subsumption_all_pre S);
   xs \<leftarrow> SPEC (\<lambda>xs. xs \<subseteq># (dom_m (get_clauses_l S)));
   (xs, S) \<leftarrow>
@@ -2618,7 +2827,7 @@ definition forward_subsumption_all :: \<open>'v twl_st_l \<Rightarrow> 'v twl_st
        else do {
          S \<leftarrow> simplify_clause_with_unit_st C S;
          if get_conflict_l S = None \<and> C \<in># dom_m (get_clauses_l S) then do {
-           S \<leftarrow> try_to_forward_subsume C S;
+           S \<leftarrow> try_to_forward_subsume no_bin C S;
            RETURN (remove1_mset C xs, S)
          }
          else RETURN (remove1_mset C xs, S)
